theories/Array.v
@@ -1,0 +1,74 @@
+Load Indexes.
+
+Inductive array {A n} :=
+  | Array : sized_list A n -> array.
+
+Arguments array : clear implicits.
+
+Definition array_to_list {A n} (a : array A n) :=
+  match a with
+  | Array sl => sized_list_to_list sl
+  end.
+
+Theorem array_to_list_length :
+  forall {A n} (a : array A n),
+  length (array_to_list a) = n.
+Proof.
+  intros ? ? ?. destruct a. apply sized_list_to_list_length.
+Qed.
+
+Definition array_empty {A} : array A 0 := Array [||].
+
+Definition array_single {A} x : array A 1 := Array [|x|].
+
+Definition array_nth {A n} i (a : array A n) :=
+  match a with
+  | Array sl => sized_list_nth i sl
+  end.
+
+Theorem array_nth_correct :
+  forall {A n} i (a : array A n),
+  array_nth i a = List.nth_error (array_to_list a) i.
+Proof.
+  intros ? ? ? ?. destruct a. apply sized_list_nth_correct.
+Qed.
+
+Definition array_update {A n} i x (a : array A n) :=
+  match a with
+  | Array sl => option_map Array (sized_list_update i x sl)
+  end.
+
+Theorem array_update_correct :
+  forall {A n} i x (a : array A n),
+  option_map array_to_list (array_update i x a) = list_update i x (array_to_list a).
+Proof.
+  intros ? ? ? ?. destruct a. unfold array_to_list, array_update. rewrite <- sized_list_update_correct.
+  destruct (sized_list_update i x s); auto.
+Qed.
+
+Definition array_push {A n} x (a : array A n) : array A (S n) :=
+  match a with
+  | Array sl => Array (sized_list_push x sl)
+  end.
+
+Theorem array_push_correct :
+  forall {A n} x (a : array A n),
+  array_to_list (array_push x a) = array_to_list a ++ [x].
+Proof.
+  intros ? ? ? ?. destruct a. apply sized_list_push_correct.
+Qed.
+
+Definition array_pop {A n} (a : array A (S n)) : array A n * A :=
+  match a with
+  | Array sl => let '(sl0, x) := (sized_list_pop sl) in (Array sl0, x)
+  end.
+
+Theorem array_pop_correct :
+  forall {A n} (a : array A (S n)),
+  (let (a0, x) := array_pop a in array_to_list a0 ++ [x]) = array_to_list a.
+Proof.
+  intros ? ? ?. destruct a. unfold array_to_list, array_pop. rewrite <- sized_list_pop_correct.
+  remember (let '(sl0, x) := sized_list_pop s in (Array sl0, x)) as sl0_x0. destruct sl0_x0 as (sl_0, x0).
+  destruct sl_0. remember (sized_list_pop s) as sl1_x1. destruct sl1_x1 as (sl1, x1).
+  injection Heqsl0_x0 as -> ->. auto.
+Qed.
